Use Pairwise more. Remove nrows from ofColumns

Tables/Data/Array/Nodup.lean
@@ -1,5 +1,7 @@
 module
 
+public import Batteries.Data.Array.Pairwise
+
 public section
 
 namespace List
@@ -15,59 +17,32 @@ end List
 namespace Array
 
 @[expose]
-def Nodup {α} (a : Array α) : Prop :=
-  ∀ i j : Nat, (_ : i < a.size) → (_ : j < a.size) → i ≠ j → a[i] ≠ a[j]
+def Nodup {α} (a : Array α) : Prop := Pairwise (fun x y => x ≠ y) a
 
 namespace Nodup
 
-abbrev Nodup' {α} (a : Array α) : Prop :=
-  ∀ i j : Fin a.size, i ≠ j → a[i] ≠ a[j]
-
-theorem iff_nodup' {α} (a : Array α) : Nodup a ↔ Nodup' a := by
-  apply Iff.intro
-  . grind [Nodup]
-  . intro h i j hi hj ne
-    exact h ⟨i, hi⟩ ⟨j, hj⟩ (by grind)
-
 instance {α} [DecidableEq α] {a : Array α}: Decidable (Nodup a) :=
-  decidable_of_iff' (Nodup' a) (iff_nodup' a)
-
-theorem empty {α} : Nodup (@empty α) := by
-  intro i j hi hj ne
-  exact (Nat.not_lt_zero i hi).elim
-
-theorem range (n : Nat) : Nodup (Array.range n) := by
-  intro i j
-  simp [Array.getElem_range]
-
-theorem finRange (n : Nat) : Nodup (Array.finRange n) := by
-  intro i j
-  simp [Array.getElem_finRange]
-
-theorem push {α} {a : Array α} {x : α} (h : Nodup a) (hfresh : x ∉ a) : Nodup (a.push x) := by
-  intro i j hi hj ne
-  simp only [getElem_push]
-  split
-  next hi =>
-    split
-    next hj => exact h i j hi hj ne
-    next hj => grind
-  next hi => grind
+  inferInstanceAs (Decidable (Pairwise (fun x y => x ≠ y) a))
 
 theorem toList_iff {α} (a : Array α) : a.Nodup ↔ a.toList.Nodup := by
-  constructor
-  . intro h
-    simp only [List.nodup_iff_pairwise_ne, ne_eq, List.pairwise_iff_getElem, length_toList,
-      getElem_toList]
-    intro i j hi hj lt
-    exact h i j hi hj (Nat.ne_of_lt lt)
-  . intro h
-    simp only [List.nodup_iff_pairwise_ne, ne_eq, List.pairwise_iff_getElem, length_toList,
-      getElem_toList] at h
-    intro i j hi hj ne
-    cases Nat.lt_or_gt_of_ne ne with
-    | inl lt => exact h i j hi hj lt
-    | inr gt => exact Ne.symm (h j i hj hi gt)
+  rfl
+
+theorem empty {α} : Nodup (@empty α) := by
+  exact pairwise_empty
+
+theorem range (n : Nat) : Nodup (Array.range n) := by
+  rw [toList_iff, Array.toList_range]
+  exact List.nodup_range
+
+theorem finRange (n : Nat) : Nodup (Array.finRange n) := by
+  rw [toList_iff, List.nodup_iff_pairwise_ne, List.pairwise_iff_getElem]
+  intro i j hi hj lt
+  simpa [Array.getElem_finRange] using Nat.ne_of_lt lt
+
+theorem push {α} {a : Array α} {x : α} (h : Nodup a) (hfresh : x ∉ a) : Nodup (a.push x) := by
+  unfold Nodup
+  rw [Array.pairwise_push]
+  exact ⟨h, by grind only⟩
 
 theorem filter {α} {a : Array α} (p : α → Bool) (h : Nodup a) : Nodup (a.filter p) := by
   rw [toList_iff, toList_filter]
