Tables/Data/Array/Pairwise.lean
@@ -1,0 +1,16 @@
+module
+
+public import Batteries.Data.Array.Pairwise
+
+public section
+
+namespace Array
+
+theorem Pairwise.filter {α} {R : α → α → Prop} {a : Array α} (p : α → Bool) (h : Pairwise R a) :
+    Pairwise R (a.filter p) := by
+  rw [Pairwise, Array.toList_filter]
+  exact List.Pairwise.filter p h
+
+end Array
+
+end
